chore: lean: continue adding withdrawals
commit-id:6464cb2e

lean/privacy/tracing/forward_tracing.lean
@@ -1,10 +1,10 @@
 import privacy.tracing.tracing
 
 structure ForwardTracing₀ where
-  (crypto: Crypto) (m: Memory) (events: List Event)
+  (crypto: Crypto) (m: Memory) (events: List (List Event))
   (context: TracingContext crypto m events)
   (note_id user_enc: ℕ)
-  (h_event: .CreateOpenNote note_id user_enc ∈ events)
+  (h_event: .CreateOpenNote note_id user_enc ∈ events.flatten)
 
 -- Decrypt the user address.
 def ForwardTracing₀.user_addr (self: ForwardTracing₀) :=
@@ -12,7 +12,7 @@ def ForwardTracing₀.user_addr (self: ForwardTracing₀) :=
 
 -- Get the user's private key.
 def ForwardTracing₀.user_priv_key (self: ForwardTracing₀) :=
-  get_priv_key self.crypto self.events self.user_addr
+  get_priv_key self.crypto self.events.flatten self.user_addr
 
 def ForwardTracing₀.user (self: ForwardTracing₀) : UserPrivKey self.crypto self.m :=
   have h := self.context.h_from_create_open_note_event self.note_id self.user_enc self.h_event
@@ -87,12 +87,186 @@ theorem ForwardTracing₁.final_coins.length (self: ForwardTracing₁) :
   unfold ForwardTracing₁.note_coins
   rw [List.length_map, List.length_finRange]
 
+def final_coin
+    {crypto: Crypto} {m: Memory} {events: List (List Event)}
+    (context: TracingContext crypto m events)
+    (coin: Coin crypto m) : Prop :=
+  ∀ (esn: ExScannedNote) (coin_idx: ℕ), context.next_coin₀ coin ≠ some (.Note esn, coin_idx)
+
+theorem ForwardTracing₁.final_coins.final (self: ForwardTracing₁)
+    (coin: Coin self.crypto self.m)
+    (h_coin: coin ∈ self.final_coins) :
+    final_coin self.context coin := by
+  by_contra h_contra
+  simp only [final_coin, not_forall] at h_contra
+  obtain ⟨esn, coin_idx, h_contra⟩ := h_contra
+  simp only [Decidable.not_not] at h_contra
+
+  simp only [ForwardTracing₁.final_coins, List.mem_map, List.mem_attach, true_and] at h_coin
+  obtain ⟨⟨coin', h_coin⟩, h_next_limit⟩ := h_coin
+  have := Graph.next_limit' (ForwardTracing₁.no_prev h_coin) |>.1
+  replace := (TracingContext.next_coin_none _ _).1 this
+
+  cases this
+  case inl h_nullifier =>
+    simp only [h_next_limit] at h_nullifier
+    have := (TracingContext.next_coin₀_from_some_note h_contra).2.2.2
+    simp [h_nullifier] at this
+  case inr this =>
+    simp [h_next_limit, h_contra] at this
+
+def coin_to_outgoing_element' {crypto: Crypto} {m: Memory} {events: List (List Event)}
+    (context: TracingContext crypto m events)
+    (coin: Coin crypto m)
+    : OutgoingElement × ℕ :=
+  match context.next_coin₀ coin with
+    | some (.Withdrawal evt, coin_idx) => (.Withdrawal evt, coin_idx)
+    | some (.Note esn, coin_idx) => (.Note esn, coin_idx)
+    | none => (.Note coin.esn, coin.coin_idx)
+
+theorem coin_to_outgoing_element'_split {crypto: Crypto} {m: Memory} {events: List (List Event)}
+    (context: TracingContext crypto m events)
+    (coin: Coin crypto m)
+    (h_final_coin: final_coin context coin) :
+    let res := coin_to_outgoing_element' context coin
+    (
+      context.next_coin₀ coin = none ∧
+      res = (.Note coin.esn, coin.coin_idx)
+    ) ∨ (
+      ∃ (evt: WithdrawalEvent) (coin_idx: ℕ),
+      context.next_coin₀ coin = some (.Withdrawal evt, coin_idx) ∧
+      res = (.Withdrawal evt, coin_idx)
+    ) := by
+  simp only [coin_to_outgoing_element']
+  split
+  · apply Or.inr
+    rename_i evt coin_idx h_next_coin₀
+    use evt, coin_idx
+  · exfalso
+    apply h_final_coin
+    assumption
+  · apply Or.inl
+    simp [*]
+
+theorem coin_to_outgoing_element'_prop {crypto: Crypto} {m: Memory} {events: List (List Event)}
+    (context: TracingContext crypto m events)
+    (coin: Coin crypto m)
+    (h_final_coin: final_coin context coin) :
+    let res := coin_to_outgoing_element' context coin
+    res.2 < res.1.amount crypto m := by
+  apply Or.elim (coin_to_outgoing_element'_split context coin h_final_coin)
+  · intro h
+    simp only [h.2, OutgoingElement.amount, coin.h_coin_idx]
+  · intro ⟨evt, coin_idx, h₀, h₁⟩
+    have := (context.next_coin₀_from_some_withdrawal h₀).2.2.1
+    simp only [OutgoingElement.amount, h₁]
+    exact this
+
+theorem coin_to_outgoing_element'_inj {crypto: Crypto} {m: Memory} {events: List (List Event)}
+    {context: TracingContext crypto m events}
+    {coin₀ coin₁: Coin crypto m}
+    (h_final_coin₀: final_coin context coin₀)
+    (h_final_coin₁: final_coin context coin₁)
+    (h_eq: coin_to_outgoing_element' context coin₀ = coin_to_outgoing_element' context coin₁) :
+    coin₀ = coin₁ := by
+  apply Or.elim (coin_to_outgoing_element'_split context coin₀ h_final_coin₀)
+  all_goals
+    intro h₀
+    apply Or.elim (coin_to_outgoing_element'_split context coin₁ h_final_coin₁)
+  all_goals
+    intro h₁
+  · simp [h₀, h₁] at h_eq
+    apply Coin.ext <;> simp [*]
+  · have ⟨_, _, h₁⟩ := h₁
+    simp [h₀, h₁] at h_eq
+  · have ⟨_, _, h₀⟩ := h₀
+    simp [h₀, h₁] at h_eq
+  · have ⟨evt₀, coin_idx₀, h₀⟩ := h₀
+    have ⟨evt₁, coin_idx₁, h₁⟩ := h₁
+    simp [h₀, h₁] at h_eq
+    simp only [h_eq] at h₀
+    exact TracingContext.next_coin₀_inj h₀.1 h₁.1
+
+def coin_to_outgoing_element {crypto: Crypto} {m: Memory} {events: List (List Event)}
+    (context: TracingContext crypto m events)
+    (coin: Coin crypto m)
+    : OutgoingElement :=
+  (coin_to_outgoing_element' context coin).1
+
+def coins_to_outgoing_elements {crypto: Crypto} {m: Memory} {events: List (List Event)}
+    (context: TracingContext crypto m events)
+    (coins: List (Coin crypto m)) : Finset OutgoingElement :=
+  coins.map (λ coin ↦ coin_to_outgoing_element context coin)
+  |>.dedup
+  |>.toFinset
+
+theorem coins_to_outgoing_elements.sum_amounts
+    {crypto: Crypto} {stxs: SuccessfulTransactions crypto}
+    (context: TracingContext crypto stxs.rm stxs.events)
+    (coins: List (Coin crypto stxs.rm))
+    (h_final_coins: ∀ coin ∈ coins, final_coin context coin) :
+    (∑ elt ∈ coins_to_outgoing_elements context coins, elt.amount crypto stxs.rm) ≥
+    coins.dedup.length := by
+  set ℓ := coins.map (coin_to_outgoing_element context) |>.dedup with h_ℓ
+
+  have := Finset.sum_list_map_count ℓ (λ elt ↦ elt.amount crypto stxs.rm)
+  rw [Finset.sum_congr rfl (by
+    intro elt h_elt
+    show _ = elt.amount crypto stxs.rm
+    rw [List.nodup_iff_count_eq_one.1 (List.nodup_dedup _), smul_eq_mul, one_mul]
+    rw [List.mem_toFinset] at h_elt
+    exact h_elt
+  )] at this
+
+  simp only [coins_to_outgoing_elements, ←h_ℓ, ←this]
+  clear this
+
+  rw [←amounts_to_coins.length]
+  set all_coins_in_notes := amounts_to_coins ℓ (λ elt ↦ elt.amount crypto stxs.rm)
+
+  let coin_to_outgoing_element'' := λ coin: { x // x ∈ coins } ↦ coin_to_outgoing_element' context ↑coin
+  have : (coins.attach).dedup.map coin_to_outgoing_element'' =
+      (coins.map (coin_to_outgoing_element' context) |>.dedup) := by
+    rw [←List.dedup_map_of_injective (by
+      intro coin₀ coin₁ h_eq
+      apply Subtype.ext
+      exact coin_to_outgoing_element'_inj (h_final_coins _ coin₀.prop) (h_final_coins _ coin₁.prop) h_eq
+    )]
+    simp [coin_to_outgoing_element'']
+
+  have : coins.dedup.length = (coins.map (coin_to_outgoing_element' context) |>.dedup |>.length) := by
+    rw [←this, List.length_map]
+    have h := List.dedup_map_of_injective Subtype.val_injective coins.attach
+    rw [List.attach_map_subtype_val] at h
+    rw [h, List.length_map]
+  rw [this]
+
+  have : all_coins_in_notes.Nodup := by
+    apply amounts_to_coins.nodup
+    exact List.nodup_dedup _
+
+  rw [←List.Nodup.dedup this]
+  rw [←List.card_toFinset, ←List.card_toFinset]
+  apply Finset.card_le_card
+  intro ⟨elt, i⟩ h_coin
+  rw [List.mem_toFinset, amounts_to_coins.mem]
+  rw [List.mem_toFinset, List.mem_map] at h_coin
+
+  replace ⟨coin, h⟩ := h_coin
+  constructor
+  · simp only [ℓ, List.mem_dedup, List.mem_map]
+    use coin, h.1
+    simp [coin_to_outgoing_element, h.2]
+  · have := coin_to_outgoing_element'_prop context coin (h_final_coins _ h.1)
+    rw [h.2] at this
+    exact this
+
 -- Given an open-note deposit, returns a list of notes that cover the note's amount.
-def forward_tracing {crypto: Crypto} {m: Memory} {events: List Event}
+def forward_tracing {crypto: Crypto} {m: Memory} {events: List (List Event)}
     (context: TracingContext crypto m events)
     (note_id user_enc: ℕ)
-    (h_event: .CreateOpenNote note_id user_enc ∈ events) :
-    Finset ExScannedNote :=
+    (h_event: .CreateOpenNote note_id user_enc ∈ events.flatten) :
+    Finset OutgoingElement :=
   let forward_tracing₀: ForwardTracing₀ := ⟨crypto, m, events, context, note_id, user_enc, h_event⟩
   match h_esn_opt: forward_tracing₀.esn_opt with
   | none =>
@@ -100,18 +274,19 @@ def forward_tracing {crypto: Crypto} {m: Memory} {events: List Event}
     .empty
   | some esn =>
     let forward_tracing₁: ForwardTracing₁ := ⟨forward_tracing₀, esn, h_esn_opt⟩
-    coins_to_notes forward_tracing₁.final_coins
+    coins_to_outgoing_elements context forward_tracing₁.final_coins
 
-theorem forward_tracing' {crypto: Crypto} {rm: ReachableMemory crypto}
-    (context: TracingContext crypto rm.m rm.events)
+theorem forward_tracing' {crypto: Crypto} {stxs: SuccessfulTransactions crypto}
+    (context: TracingContext crypto stxs.rm.m stxs.events)
     (note_id user_enc: ℕ)
-    (h_event: .CreateOpenNote note_id user_enc ∈ rm.events) :
-    let forward_tracing₀: ForwardTracing₀ := ⟨crypto, rm.m, rm.events, context, note_id, user_enc, h_event⟩
+    (h_event: .CreateOpenNote note_id user_enc ∈ stxs.events.flatten) :
+    let forward_tracing₀: ForwardTracing₀ := ⟨crypto, stxs.rm.m, stxs.events, context, note_id, user_enc, h_event⟩
     ∃ esn, ∃ h: forward_tracing₀.esn_opt = some esn,
       let forward_tracing₁: ForwardTracing₁ := ⟨forward_tracing₀, esn, h⟩
       forward_tracing context note_id user_enc h_event =
-      (coins_to_notes forward_tracing₁.final_coins) := by
+      (coins_to_outgoing_elements context forward_tracing₁.final_coins) := by
   intro forward_tracing₀
+  rw [SuccessfulTransactions.events.flatten_eq] at h_event
   have ⟨inp, note_imp, h_note_id, h_r, h_user_enc⟩ := NoteImplies.from_open_note_event h_event
 
   have h_addrbob : forward_tracing₀.user_addr = inp.addrbob := by
@@ -124,13 +299,13 @@ theorem forward_tracing' {crypto: Crypto} {rm: ReachableMemory crypto}
     simp only [forward_tracing₀] at h_addrbob
 
     let register_imp₀ := note_imp.subchannel.channel.bob_registered
-    have register_imp₁ := RegisterImplies.for_get_priv_key rm inp.addrbob (by
+    have register_imp₁ := RegisterImplies.for_get_priv_key stxs.rm inp.addrbob (by
       simp [register_imp₀.public_key]
       exact crypto.zero_not_public_key ⟨_, register_imp₀.h_kalice⟩
     )
     have := register_imp₁.public_key ▸ register_imp₀.public_key
     apply crypto.priv_to_pub_inj (forward_tracing₀.user.k.prop) register_imp₀.h_kalice
-    simp only [←h_addrbob] at this
+    simp only [←h_addrbob, ←SuccessfulTransactions.events.flatten_eq] at this
     exact this
   have : forward_tracing₀.user.k = kbob := by
     apply Subtype.ext; exact this
@@ -171,54 +346,95 @@ theorem forward_tracing' {crypto: Crypto} {rm: ReachableMemory crypto}
     exact Option.some.inj (h_esn_opt ▸ h_esn_opt')
 
 theorem forward_tracing_props
-    {crypto: Crypto} {rm: ReachableMemory crypto}
-    (context: TracingContext crypto rm.m rm.events)
+    {crypto: Crypto} {stxs: SuccessfulTransactions crypto}
+    (context: TracingContext crypto stxs.rm.m stxs.events)
     (note_id user_enc: ℕ)
-    (h_event: .CreateOpenNote note_id user_enc ∈ rm.events) :
-    let output_notes := forward_tracing context note_id user_enc h_event
-    (∀ esn' ∈ output_notes,
-      rm.m .Notes [esn'.note_id crypto, 0] ≠ 0 ∧
-      rm.m .Nullifiers [crypto.hash [esn'.c, esn'.token, esn'.i, get_priv_key crypto rm.events esn'.addrbob]] = 0
+    (h_event: .CreateOpenNote note_id user_enc ∈ stxs.events.flatten) :
+    let outputs := forward_tracing context note_id user_enc h_event
+    (∀ elt ∈ outputs,
+      match elt with
+      | .Note esn' =>
+        stxs.rm.m .Notes [esn'.note_id crypto, 0] ≠ 0 ∧
+        stxs.rm.m .Nullifiers [crypto.hash [esn'.c, esn'.token, esn'.i, get_priv_key crypto stxs.events.flatten esn'.addrbob]] = 0
+      | .Withdrawal evt =>
+        Event.Withdraw evt.user_enc evt.amount evt.token ∈ stxs.events.flatten
     ) := by
   have ⟨esn, h_esn_opt, h_forward_tracing⟩ := forward_tracing' context note_id user_enc h_event
   rw [h_forward_tracing]
   dsimp only
-  set forward_tracing₀: ForwardTracing₀ := ⟨crypto, rm.m, rm.events, context, note_id, user_enc, h_event⟩ with h_forward_tracing₀
+  set forward_tracing₀: ForwardTracing₀ := ⟨crypto, stxs.rm.m, stxs.events, context, note_id, user_enc, h_event⟩ with h_forward_tracing₀
+  let forward_tracing₁: ForwardTracing₁ := ⟨forward_tracing₀, esn, h_esn_opt⟩
 
-  intro esn' h_esn'
-  simp only [coins_to_notes, List.mem_toFinset, List.mem_dedup, List.mem_map] at h_esn'
-  replace ⟨coin, h_coin, h_esn'⟩ := h_esn'
-  simp only [ForwardTracing₁.final_coins, List.mem_map, List.mem_attach] at h_coin
-  replace ⟨⟨coin', h_coin⟩, _, h_next_limit⟩ := h_coin
-  have := (context.tracing_graph.next_limit' (ForwardTracing₁.no_prev h_coin)).1
-  rw [h_next_limit] at this
-  replace := (context.next_coin_none coin).1 this
-  simp only [h_esn', TracingContext.bob] at this
+  intro elt h_elt
 
-  refine ⟨?_, this⟩
-  · have ⟨inp, note_imp, h_note_id⟩ := NoteImplies.from_coin coin
-    have := note_imp.h_note_exists
-    rw [note_exists, h_note_id] at this
-    rw [←h_esn']
-    exact this
+  simp only [coins_to_outgoing_elements, List.mem_toFinset, List.mem_dedup, List.mem_map] at h_elt
+  replace ⟨coin, h_elt⟩ := h_elt
+  have h_final := ForwardTracing₁.final_coins.final forward_tracing₁ coin h_elt.1
+  simp only [ForwardTracing₁.final_coins, List.mem_map, List.mem_attach, true_and] at h_elt
+
+  cases elt
+  case Note esn' =>
+    replace ⟨⟨⟨coin', h_coin⟩, h_next_limit⟩, h_elt⟩ := h_elt
+    have := (Graph.next_limit' (ForwardTracing₁.no_prev h_coin)).1
+    rw [h_next_limit] at this
+    replace := (context.next_coin_none coin).1 this
+    simp only [TracingContext.bob] at this
+    cases this
+    case inr this =>
+      replace ⟨_, _, this⟩ := this
+      simp [coin_to_outgoing_element, coin_to_outgoing_element', this] at h_elt
+    case inl this =>
+      have h_esn' : coin.esn = esn' := by
+        simp only [coin_to_outgoing_element] at h_elt
+        apply Or.elim (coin_to_outgoing_element'_split context coin h_final)
+        · intro h
+          simp only [h.2, OutgoingElement.Note.injEq] at h_elt
+          exact h_elt
+        · intro ⟨_, _, h⟩
+          simp [h.2] at h_elt
+
+      refine ⟨?_, ?_⟩
+      · have ⟨inp, note_imp, h_note_id⟩ := NoteImplies.from_coin coin
+        have := note_imp.h_note_exists
+        rw [note_exists, h_note_id] at this
+        rw [←h_esn']
+        exact this
+      · rwa [←h_esn']
+
+  case Withdrawal evt =>
+    simp only
+
+    apply Or.elim (coin_to_outgoing_element'_split context coin h_final)
+    · intro h
+      simp [coin_to_outgoing_element, h.2] at h_elt
+    · intro ⟨evt', coin_idx, h⟩
+      simp only [coin_to_outgoing_element, h.2, OutgoingElement.Withdrawal.injEq] at h_elt
+      simp [h_elt.2] at h
+      exact (context.next_coin₀_from_some_withdrawal h.1).2.2.2
 
 theorem forward_tracing_sum_amounts
-    {crypto: Crypto} {rm: ReachableMemory crypto}
-    (context: TracingContext crypto rm.m rm.events)
+    {crypto: Crypto} {stxs: SuccessfulTransactions crypto}
+    (context: TracingContext crypto stxs.rm.m stxs.events)
     (note_id user_enc: ℕ)
-    (h_event: .CreateOpenNote note_id user_enc ∈ rm.events) :
-    let output_notes := forward_tracing context note_id user_enc h_event
-    ∑ esn ∈ output_notes, esn.amount crypto rm ≥ (crypto.unpack (rm.m .Notes [note_id, 0])).2 := by
+    (h_event: .CreateOpenNote note_id user_enc ∈ stxs.events.flatten) :
+    let outputs := forward_tracing context note_id user_enc h_event
+    ∑ elt ∈ outputs, elt.amount crypto stxs.rm ≥ (crypto.unpack (stxs.rm.m .Notes [note_id, 0])).2 := by
   have ⟨esn, h_esn_opt, h_forward_tracing⟩ := forward_tracing' context note_id user_enc h_event
-  rw [h_forward_tracing]
-  intro output_notes
+  simp only [h_forward_tracing]
 
-  apply le_trans _ (coins_to_notes.sum_amounts _)
+  apply le_trans _ (coins_to_outgoing_elements.sum_amounts context _ (by
+    intro coin h_coin
+    let forward_tracing₀: ForwardTracing₀ := ⟨crypto, stxs.rm.m, stxs.events, context, note_id, user_enc, h_event⟩
+    let forward_tracing₁: ForwardTracing₁ := ⟨forward_tracing₀, esn, h_esn_opt⟩
+    exact ForwardTracing₁.final_coins.final forward_tracing₁ coin h_coin
+  ))
+
   rw [List.Nodup.dedup (ForwardTracing₁.final_coins.nodup _)]
   rw [ForwardTracing₁.final_coins.length]
 
-  set forward_tracing₀: ForwardTracing₀ := ⟨crypto, rm.m, rm.events, context, note_id, user_enc, h_event⟩ with h_forward_tracing₀
+  set forward_tracing₀: ForwardTracing₀ := ⟨crypto, stxs.rm.m, stxs.events, context, note_id, user_enc, h_event⟩ with h_forward_tracing₀
   let forward_tracing₁: ForwardTracing₁ := ⟨forward_tracing₀, esn, h_esn_opt⟩
+  rw [SuccessfulTransactions.events.flatten_eq] at h_event
   have ⟨inp, note_imp, h_note_id, h_r⟩ := NoteImplies.from_open_note_event h_event
 
   have : esn.note_id crypto = inp.note_id crypto := by
