lean/privacy/actions.lean
@@ -3,3 +3,4 @@ import privacy.actions.info
 import privacy.actions.reachable_memory
 import privacy.actions.run_action
 import privacy.actions.server_actions
+import privacy.actions.withdrawals
